Extract a (not yet active) validator test

tests/Test.fst
@@ -9,8 +9,55 @@ open FStar.Bytes
 module CH = QD.Parse_clientHello
 module SH = QD.Parse_serverHello
 module NST = QD.Parse_newSessionTicket
+module B = LowStar.Buffer
+module LP = LowParse.Low.Base
+module I32 = FStar.Int32
+module HST = FStar.HyperStack.ST
+module LT = LowParse.TestLib.Low
 
-let main () : St C.exit_code =
+#set-options "--z3rlimit 16"
+
+let test_validate_aux
+  (client_hello: LP.buffer8)
+  (client_hello_len: I32.t { I32.v client_hello_len == B.length client_hello } )
+  (server_hello: LP.buffer8)
+  (server_hello_len: I32.t { I32.v server_hello_len == B.length server_hello } )
+  (new_session_ticket: LP.buffer8)
+  (new_session_ticket_len: I32.t { I32.v new_session_ticket_len == B.length new_session_ticket } )
+: HST.Stack C.exit_code
+  (requires (fun h -> B.live h client_hello /\ B.live h server_hello /\ B.live h new_session_ticket))
+  (ensures (fun h _ h' -> B.modifies B.loc_none h h'))
+= print (!$"Validating client hello...");
+  let r = CH.clientHello_validator32 client_hello client_hello_len in
+  if r `I32.lt` 0l
+  then
+    let _ = print (!$"failed.\n") in
+    C.EXIT_FAILURE
+  else
+//    let _ = print_string ("OK, validated " ^ I32.to_string (client_hello_len `I32.sub` r) ^ " bytes\n") in
+    let r = SH.serverHello_validator32 server_hello server_hello_len in
+    if r `I32.lt` 0l
+    then
+      let _ = print (!$"failed.\n") in
+      C.EXIT_FAILURE
+    else
+//      let _ = print_string ("OK, validated " ^ I32.to_string (server_hello_len `I32.sub` r) ^ " bytes\n") in
+      let r = NST.newSessionTicket_validator32 new_session_ticket new_session_ticket_len in
+      if r `I32.lt` 0l
+      then
+        let _ = print (!$"failed.\n") in
+        C.EXIT_FAILURE
+      else
+//        let _ = print_string ("OK, validated " ^ I32.to_string (new_session_ticket_len `I32.sub` r) ^ " bytes\n") in
+        C.EXIT_SUCCESS
+
+let test_validate () : St C.exit_code =
+  let (client_hello, client_hello_len) = LT.load_file_buffer "test_client_hello.input" in
+  let (server_hello, server_hello_len) = LT.load_file_buffer "test_server_hello.input" in
+  let (new_session_ticket, new_session_ticket_len) = LT.load_file_buffer "test_new_session_ticket.input" in
+  test_validate_aux client_hello client_hello_len server_hello server_hello_len new_session_ticket new_session_ticket_len
+
+let test_parse () : St C.exit_code =
   let client_hello = bytes_of_hex "0303636fad80506049a41bf5d2bc6282def8541c064f7c5dfc1a22d15d1fdb63a7312053bada022607152b1f61edc26aa42ae04e47a557188d8d5618aa43fed2bfe358003e130213031301c02cc030009fcca9cca8ccaac02bc02f009ec024c028006bc023c0270067c00ac0140039c009c0130033009d009c003d003c0035002f00ff010000b2000000190017000014746c7331332e636c6f7564666c6172652e636f6d000b000403000102000a000c000a001d0017001e00190018002300000016000000170000000d0030002e040305030603080708080809080a080b080408050806040105010601030302030301020103020202040205020602002b0009087f1c030303020301002d00020101003300260024001d002028f6c297892591276bf0dd77a6c1ade6b586ed955e80dc79c3bb98609f538101" in
   let server_hello = bytes_of_hex (* record header "02000076" *) "0303f71ed30cc04779b506a9f8af668da1b5fd8f26357c12cd4ba7c214f680e14e0f20c01886bb135f6d36102340ca06c5f9b9b777438dc3dda56e747003216dcbf136130200002e00330024001d0020b4871c8695fc4be0eae36067356ee16ff5e92e756f89b2cbfe48525acd3e0c27002b00027f1c" in
   let new_session_ticket = bytes_of_hex "0002a3002af9a838010000d08225ecc6fec0ee18c3dfef6d54a87f1d742ee5a43abbe59a3c86441dbd5ad39e69320a025e89481d3c7ee6b199bf944a8f4834b4d39da4706445ee8b0ea43b910bde77faffde5f856c906932dbe75bd60aa5f9c7b5ec47735e9f2deadf28828801ba2484b9a8cb5e7861d63840723fb9182d4db9cc1e91057949df74161360ae06b4ebf38f7611c36406808d4060d43c82888794b6c8d2a6d32aa16eafd9fd01b5fbaf7a8924d6b502f8f1898f6413845855a03e5ff7273402f85e1269d26298bd8a00512c0d8e45c005f06c200a52200008002a000400003800" in
@@ -20,20 +67,21 @@ let main () : St C.exit_code =
     print (!$"failed.\n");
     C.EXIT_FAILURE
   | Some (ch, r) ->
-    print_string ("OK, parsed "^(FStar.UInt32.to_string r)^" bytes\n");
+//    print_string ("OK, parsed "^(FStar.UInt32.to_string r)^" bytes\n");
     print (!$"Parsing server hello... ");
     match SH.serverHello_parser32 server_hello with
     | None ->
       print (!$"failed.\n");
       C.EXIT_FAILURE
     | Some (sh, r) ->
-      print_string ("OK, parsed "^(FStar.UInt32.to_string r)^" bytes\n");
+//      print_string ("OK, parsed "^(FStar.UInt32.to_string r)^" bytes\n");
       print (!$"Parsing new session ticket... ");
       match NST.newSessionTicket_parser32 new_session_ticket with
       | None ->
         print (!$"failed.\n");
 	C.EXIT_FAILURE
       | Some (nst, r) ->
-        print_string ("OK, parsed "^(FStar.UInt32.to_string r)^" bytes\n");
+//        print_string ("OK, parsed "^(FStar.UInt32.to_string r)^" bytes\n");
         C.EXIT_SUCCESS
 
+let main () : St C.exit_code = test_parse ()
